feat(*) add examples to paper theory

Paper/Paper.thy
@@ -1,22 +1,22 @@
 (*<*)
 theory Paper
-  imports Syntax
+  imports "HOL_To_IMP_Refinements.HOL_To_IMP_Minus_Lists" Syntax
 begin
 (*>*)
 
 text \<open>
-  This is the alignment theory for the paper: 
-  
+  This is the alignment theory for the paper:
+
   "Proof-Producing Translation of Functional Programs into a Time & Space Reasonable Model"
-  
+
   Open this file in Isabelle/jEdit, as described in the supplied README.
-  Formal elements referenced in the texts are all clickable to see the original definition.
+  Formal elements referenced in the texts are all clickable, leading to the original definition.
   To get the statements as close to the informal text as possible, local notation is introduced,
   and implicit assumptions are stated via local context where necessary.
 \<close>
 
 section \<open>Preliminaries\<close>
-                                
+
 text \<open>Registers are of @{typ vname}, values of @{typ val}, state of @{typ state}.\<close>
 
 text \<open>Atom evaluation function @{const atomVal} with the following equations:\<close>
@@ -30,14 +30,14 @@ text \<open>Expression evaluation function @{const aval} with the following equa
 lemma "\<lbrakk>A\<^sub>1 + A\<^sub>2\<rbrakk>\<^sub>s = \<lbrakk>A\<^sub>1\<rbrakk>\<^sub>s + \<lbrakk>A\<^sub>2\<rbrakk>\<^sub>s" by simp
 lemma "\<lbrakk>A\<^sub>1 - A\<^sub>2\<rbrakk>\<^sub>s = \<lbrakk>A\<^sub>1\<rbrakk>\<^sub>s - \<lbrakk>A\<^sub>2\<rbrakk>\<^sub>s" by simp
 
-subsection \<open>Big-step semantics\<close>
+subsection \<open>Execution Relation (Big-Step Semantics)\<close>
 text \<open>
-  Commands also contain a no-op command ("SKIP") for technical reasons, which we skip in the paper
-  as it is irrelevant. Shared rules (here from @{const big_step_t}):
+  Commands also contain a no-op command (@{const SKIP}) for technical reasons, which we skip in the
+  paper as it is irrelevant. Here are the shared rules (from @{const big_step_t}):
 \<close>
-(*<*)unbundle no atom unbundle no aops unbundle orig(*>*)
+(*<*)unbundle no atom unbundle no aops unbundle orig and no big_step_syntax and no tbig_step_syntax (*>*)
 
-lemma Assign: 
+lemma Assign:
   assumes "s' = s(r := \<lbrakk>a\<rbrakk>\<^sub>s)"
   shows "(r ::= a, s) \<Rightarrow>\<^bsup>2\<^esup> s'"
 (*<*)using assms by (auto simp: numeral_eq_Suc)(*>*)
@@ -54,13 +54,13 @@ lemma IfF:
 
 lemma Seq:
   assumes "(p\<^sub>1,s) \<Rightarrow>\<^bsup>n\<^sub>1\<^esup> s'" "(p\<^sub>2,s') \<Rightarrow>\<^bsup>n\<^sub>2\<^esup> s''"
-    shows "(p\<^sub>1;;p\<^sub>2,s) \<Rightarrow>\<^bsup>n\<^sub>1+n\<^sub>2+0\<^esup> s''" 
+    shows "(p\<^sub>1;;p\<^sub>2,s) \<Rightarrow>\<^bsup>n\<^sub>1+n\<^sub>2+0\<^esup> s''"
 (*<*)using assms by auto(*>*)
 
 subsection "Theorem 1"
 
 text \<open>
-\<open>a\<^bsub>max\<^esub>\<close> via @{const max_const} typeclass. The theorem @{thm IMP_space_growth} also needs the
+\<open>a\<^bsub>max\<^esub>\<close> via @{class max_const} typeclass. The theorem @{thm IMP_space_growth} also needs the
 implicit assumption that the state has a finite codomain.\<close>
 
 context fixes s :: state assumes "finite (range s)" begin
@@ -88,13 +88,88 @@ text \<open>TODO link selector\<close>
 text \<open>TODO another example\<close>
 text \<open>TODO link to ML structure\<close>
 
-section \<open>\<open>HOL\<^bsup>TC\<nat>\<close> to \<open>IMP\<^bsup>TC\<^esup>\<close>\<close>
+section \<open>\<open>HOL\<^bsup>(TC)\<^esup>\<close> to \<open>HOL\<^bsup>(TC)\<nat>\<^esup>\<close>\<close>
+
+subsection "Theorem 3"
+
+lemma "galois.galois_equivalence (=\<^bsub>range (natify :: 'a :: compile_nat  \<Rightarrow> _)\<^esub>) ((=) :: 'a \<Rightarrow> _)
+  denatify natify"
+(*<*) by (fact compile_nat_type_def.galois_equivalence) (*>*)
+
+subsection \<open>Example 3 (Appendix)\<close>
+
+text \<open>The type of lists is already compiled (see @{const Cons_nat}).
+For illustration purposes, we compile a copy of the type:\<close>
+
+datatype 'a listcopy = Nil_copy | Cons_copy 'a "'a listcopy"
+datatype_compile_nat listcopy
+print_theorems (*move your cursor on the command to the left to see all generated theorems and constants*)
+
+subsection \<open>Fig. 4\<close>
+
+context HOL_To_HOL_Nat
+begin
+
+text \<open>The synthesis is fully automatic. We list the corresponding theorems from the figure below.
+Here is the input function:\<close>
+
+fun count_acc' :: "'a \<Rightarrow> 'a list \<Rightarrow> nat \<Rightarrow> nat" where
+  "count_acc' a [] n = n"
+| "count_acc' a (x#xs) n = count_acc' a xs (if x = a then Suc n else n)"
+(*<*) declare count_acc'.simps[simp del] (*>*)
+
+text \<open>First, get a single equation (Listing 1.1):\<close>
+
+case_of_simps count_acc'_eq : count_acc'.simps
+
+text \<open>Now we use black-box and white-box transport to obtain the related constant and its
+defining, tail-recursive equation:\<close>
+
+function_compile_nat count_acc'_eq
+print_theorems (*move your cursor on the command to the left to see all generated theorems and constants*)
+
+text \<open>Related constant from black-box transport (Listing 1.2):\<close>
+
+lemma "(Rel_nat ===> Rel_nat ===> Rel_nat ===> Rel_nat) (count_acc'_nat TYPE('a :: compile_nat))
+  (count_acc' :: 'a \<Rightarrow> _)"
+(*<*) by (fact count_acc'_related_transfer) (*>*)
+
+text \<open>Theorem from white-box transport (Listing 1.3):\<close>
+
+lemma
+  assumes "Rel_nat a (a' :: 'a :: compile_nat)"
+  and "Rel_nat xs (xs' :: 'a list)"
+  and "Rel_nat n (n' :: nat)"
+  shows "Rel_nat
+    (case_list_nat n
+      (\<lambda>x xs. count_acc'_nat TYPE('a) a xs (if x = a then Suc n else n))
+      xs)
+    (count_acc' a' xs' n')"
+(*<*) using assms Rel_nat_count_acc'_nat_unfolded[unfolded If_nat_def eq_nat_eq_False_nat_iff]
+  by fastforce (*>*)
+
+text \<open>Final tail-recursive equation (Listing 1.4), using that @{const Rel_nat} is left-unique,
+as shown in @{thm left_unique_Rel_nat}:\<close>
+
+lemma
+  assumes "Rel_nat a (a' :: 'a :: compile_nat)"
+  and "Rel_nat xs (xs' :: 'a list)"
+  and "Rel_nat n (n' :: nat)"
+  shows "count_acc'_nat TYPE('a) a xs n =
+    case_list_nat n (\<lambda>x xs. count_acc'_nat TYPE('a) a xs (if x = a then Suc n else n)) xs"
+(*<*) using assms count_acc'_nat_eq_unfolded[unfolded If_nat_def eq_nat_eq_False_nat_iff]
+  by fastforce (*>*)
+
+end
+
+
+section \<open>\<open>HOL\<^bsup>TC\<nat>\<^esup>\<close> to \<open>IMP\<^bsup>TC\<^esup>\<close>\<close>
 
 subsection \<open>Fig. 5\<close>
 text \<open>Commands as @{typ tcom}, semantics via @{const tbig_step_t}. Special rules:\<close>
 (*<*)unbundle tcom_syntax unbundle partial(*>*)
 
-lemma Call: 
+lemma Call:
   assumes "(pc,s) \<Rightarrow>\<^sub>r\<^bsup>n\<^esup> v" "s' = s(r := v)"
   shows "p \<turnstile> (CALL pc RETURN r,s) \<Rightarrow>\<^bsup>n+0\<^esup> s'"
   (*<*)using assms by auto(*>*)
@@ -103,6 +178,70 @@ lemma Rec:
   assumes "p \<turnstile> (p,s) \<Rightarrow>\<^bsup>n\<^esup> s'"
   shows "p \<turnstile> (RECURSE,s) \<Rightarrow>\<^bsup>n+5\<^esup> s'"
   (*<*)using assms by (metis add.commute tTail)(*>*)
+
+subsection \<open>Example 1\<close>
+
+text \<open>See @{thm HOL_To_HOL_Nat.fun_pow_snd_nat_eq}.\<close>
+
+subsection \<open>Compilation to \<open>IMP\<^bsup>TC\<^esup>\<close>\<close>
+
+text \<open>See @{ML_structure Compile_HOL_Nat_To_IMP}.\<close>
+
+subsection \<open>Execution Rules used for Symbolic Execution of \<open>IMP\<^bsup>TC\<^esup>\<close> Programs (Fig. 14, Appendix)\<close>
+
+(*TODO, see terminates_with_res_tSeqI and below*)
+
+subsection \<open>Example 2\<close>
+
+context HOL_Nat_To_IMP_Minus
+begin
+
+text \<open>First, unfold the case combinator to if-then-elses:\<close>
+
+lemmas count_acc'_nat_eq = HTHN.count_acc'_nat_eq_unfolded[unfolded case_list_nat_def]
+
+text \<open>Then, generate the \<open>IMP\<^bsup>TC\<^esup>\<close> program:\<close>
+
+compile_nat (non-optimized) count_acc'_nat_eq (*remove the non-optimized flag for a shorter program*)
+
+text \<open>Then, prove the correctness. This is fully automatic, using the method @{method cook}.
+Here, we pr
+Here, we provide the corresponding
+step-by-step proof from the paper. Here is the input function:
+\<close>
+
+HOL_To_IMP_Minus_correct HOL_To_HOL_Nat.count_acc'_nat
+  text \<open>We prove correctness of the compiled \<open>IMP\<^bsup>W\<^esup>\<close> program. First, we reduce this proof to the
+  correctness proof of the generated \<open>IMP\<^bsup>TC\<^esup>\<close> program.\<close>
+  apply (tactic \<open>HM.correct_if_IMP_tailcall_correct_tac HT.get_IMP_def @{context} 1\<close>)
+  text \<open>Initial goal (Listing 1.5)\<close>
+  apply (tactic \<open>HT.setup_induction_tac HT.get_fun_inducts @{context} 1\<close>) defer
+  text \<open>Cons-case (Listing 1.6)\<close>
+  apply (tactic \<open>HT.start_case_tac HT.get_IMP_def @{context} 1\<close>)
+  apply (tactic \<open>HT.run_tac HT.get_imp_minus_correct @{context} 1\<close>)
+  apply (tactic \<open>HT.run_HOL_fun_tac HB.get_HOL_eqs @{context} 1\<close>)
+  text \<open>Goals after symbolic execution (Listing 1.7)\<close>
+  apply (tactic \<open>HT.apply_IH_tac @{context} 1\<close>)
+  text \<open>Relatedness goals after application of inductive hypothesis (Listing 1.8)\<close>
+  apply (tactic \<open>HT.solve_IH_prem_tac @{context} 1\<close>)
+  apply (tactic \<open>HT.solve_IH_prem_tac @{context} 1\<close>)
+  apply (tactic \<open>HT.solve_IH_prem_tac @{context} 1\<close>)
+  text \<open>Second subcase in Cons-case\<close>
+  apply (tactic \<open>HT.finish_tac HB.get_HOL_eqs @{context} 1\<close>)
+  text \<open>Nil-case\<close>
+  apply (tactic \<open>HT.start_case_tac HT.get_IMP_def @{context} 1\<close>)
+  apply (tactic \<open>HT.run_tac HT.get_imp_minus_correct @{context} 1\<close>)
+  apply (tactic \<open>HT.finish_tac HB.get_HOL_eqs @{context} 1\<close>)
+  text \<open>Done! We do not close the proof because in the next command, we prove it again, automatically:\<close>
+  oops
+
+HOL_To_IMP_Minus_correct HOL_To_HOL_Nat.count_acc'_nat by cook
+
+end
+
+subsection \<open>Case Studies\<close>
+
+text \<open>Can be found in @{dir "../HOL_To_IMP-/Refinements"}.\<close>
 
 
 section \<open>\<open>IMP\<^bsup>TC\<^esup>\<close> to \<open>IMP\<^sup>-\<close>\<close>
@@ -191,7 +330,7 @@ theorem "p \<turnstile> (p,s) \<Rightarrow>\<^bsub>regs p\<^esub>\<^bsup>n\<^esu
 (*<*)
   apply standard
   subgoal
-    using compile_sound[OF _ \<open>invar p\<close>]  unfolding eq_on_def 
+    using compile_sound[OF _ \<open>invar p\<close>]  unfolding eq_on_def
     apply (auto intro: le_trans add_le_cancel_right)
     apply (smt (verit) add_le_cancel_right le_trans add.commute)
     done
@@ -208,7 +347,7 @@ end
 subsection "Lemma 2"
 text \<open>Lemma in @{thm neat_subst}.\<close>
 
-lemma 
+lemma
   assumes "inj m"
     shows "(p[(m x)/x],s)\<Rightarrow>\<^bsup>n\<^esup> s' \<Longrightarrow> (p,s o m)\<Rightarrow>\<^bsup>n\<^esup> s' o m"
   (*<*)using assms neat_subst by auto(*>*)
@@ -216,7 +355,7 @@ lemma
 
 subsection "Theorem 7"
 text \<open>
-  Definition in @{const inline}, correctness theorems @{thm inline_sound} 
+  Definition in @{const inline}, correctness theorems @{thm inline_sound}
   and @{thm inline_complete}
 \<close>
 (*<*)(*>*)
@@ -226,8 +365,8 @@ theorem "(p,s)\<Rightarrow>\<^bsub>regs p\<^esub>\<^bsup>n\<^esup> s' \<Longrigh
 proof -
   assume "(p,s)\<Rightarrow>\<^bsub>regs p\<^esub>\<^bsup>n\<^esup> s'"
   then obtain n' s'' where "n' \<le> n" and s'': "big_step_t' (p,s) n' s''" "s'' = s' on set (regs p)" by blast
-  from inline_sound[OF this(2)] obtain z t where 
-    t: "big_step_t (\<lparr>p\<rparr>\<^sub>\<star>, s) z t" "t = s'' on set (regs p)" and 
+  from inline_sound[OF this(2)] obtain z t where
+    t: "big_step_t (\<lparr>p\<rparr>\<^sub>\<star>, s) z t" "t = s'' on set (regs p)" and
     z: "n' \<le> z" "z \<le> (n'+1)*(1+\<bar>p\<bar>)"
     by blast
   from z \<open>n' \<le> n\<close> have "z \<le> (n+1)*(\<bar>p\<bar>+1)"
@@ -282,7 +421,7 @@ subsection "Lemma 3"
 text \<open>Adder in @{const binary_adder}, lemma in @{thm assignment_to_binary_correct}\<close>
 (*<*)unbundle no minus unbundle minus2(*>*)
 
-context 
+context
   fixes w::nat assumes "0 < w"
   fixes s::state assumes "finite (range s)"
 begin
@@ -311,7 +450,7 @@ theorem
 (*<*)
 proof -
   from assms(1) obtain n' where *: "big_step_t (p,s) n' s'" "n' \<le> n" by blast
-  with assms have **: "n' < w" "2 ^ n' * (omax (s\<^bsub>max \<^esub>) (p\<^bsub>max\<^esub>)) < 2 ^ w" 
+  with assms have **: "n' < w" "2 ^ n' * (omax (s\<^bsub>max \<^esub>) (p\<^bsub>max\<^esub>)) < 2 ^ w"
     apply auto
     using Orderings.preorder_class.dual_order.strict_trans2
     by fastforce
